lean-tracing-demo-ccfraft/Sparse.lean
@@ -29,6 +29,7 @@ import Sparse.LogMatchEncoding
 import Sparse.MonotoneIntervals
 import Sparse.NativeArrayCheckQuorum
 import Sparse.NativeArrayQueue
+import Sparse.NativeArrayVote
 import Sparse.NativeConstructors
 import Sparse.NativeNodeOperations
 import Sparse.NativeNodeSets
